\titledquestion{Compare and Proof}

For each pair of functions \(f(n)\) and \(g(n)\), give your answer whether \(f(n) = o(g(n))\), \(f(n) = \omega(g(n))\) or \(f(n) = \Theta(g(n))\).  Give a \textbf{proof} of your answers.

\begin{parts}
    \part[3] \par
    \[f(n) = \log(n!)\]
    \[g(n) = \log(n^n)\]

    \begin{solution}
        $f(n) = \Theta(g(n))$
        \begin{align*}
            \lim_{n\to\infty} \frac{f(n)}{g(n)} & = \lim_{n\to\infty} \frac{\log(n!)}{\log(n^n)}                                                    \\
                                                & = \lim_{n\to\infty} \frac{\log(n!)}{n\log(n)}                                                     \\
                                                & = \lim_{n\to\infty} \frac{n\log{n} - n\log{e} + O(\log{n})}{n\log{n}}\ \ (Strling\ approximation) \\
                                                & = \lim_{n\to\infty} \frac{n\log{\frac{n}{e}} + O(\log{n})}{n\log{n}}                              \\
                                                & = 1
        \end{align*}

        Since $0 < 1 < \infty$, $f(n) = \omega(g(n)),\  f(n) = \Theta(g(n))$



    \end{solution}
    \newpage
    \part[3] \par
    \[f(n) = n^{1+\varepsilon}, \qquad (\varepsilon\in \mathbb{R}^+)\]
    \[g(n) = n(\log n)^k, \qquad (k\in \mathbb{Z}^+)\]

    \begin{solution}
        $f(n) = \omega(g(n))$
        \begin{align*}
            \lim_{n\to\infty} \frac{f(n)}{g(n)} & = \lim_{n\to\infty} \frac{n^{1+\varepsilon}}{n(\log n)^k}                                                                   \\
                                                & = \lim_{n\to\infty} \frac{n^{\varepsilon}}{(\log n)^k}                                                                      \\
                                                & = \lim_{n\to\infty} \frac{\varepsilon n^{\varepsilon - 1}}{k(\log n)^{k-1} \frac{1}{n \ln{2}}}          & \quad (L'Hopital's rule) \\
                                                & = \lim_{n\to\infty} \frac{\ln(2) \varepsilon n^{\varepsilon}}{k(\log n)^{k-1}}                                                  \\
                                                & = \lim_{n\to\infty} \frac{\ln(2) \varepsilon^2 n^{\varepsilon - 1}}{k(k-1)(\log n)^{k-2} \frac{1}{n \ln(2)}}   & \quad (L'Hopital's rule) \\
                                                & = \lim_{n\to\infty} \frac{(\ln(2) \varepsilon)^2 n^{\varepsilon}}{k(k-1)(\log n)^{k-2}}                                              \\
                                                & \quad \vdots                                                                                                                \\
                                                & = \lim_{n\to\infty} \frac{(ln(2) \varepsilon)^{k-1} n^{\varepsilon}}{k!(\log n)}                                                    \\
                                                & = \lim_{n\to\infty} \frac{(ln(2) \varepsilon)^{k} n^{\varepsilon}}{k!}                                   & \quad (L'Hopital's rule) \\
                                                & = \infty
        \end{align*}
    \end{solution}

\end{parts}
